moved operators to specific file instead of common file

common/Values.v
@@ -767,61 +767,6 @@ Definition rolml (v: val) (amount: int) (mask: int64): val :=
   end.
 
 
-Definition extfz stop start v :=
-  if (Z.leb start stop)
-       && (Z.geb start Z.zero)
-       && (Z.ltb stop Int.zwordsize)
-  then
-    let stop' := Z.add stop Z.one in
-    match v with
-    | Vint w =>
-      Vint (Int.shru (Int.shl w (Int.repr (Z.sub Int.zwordsize stop'))) (Int.repr (Z.sub Int.zwordsize (Z.sub stop' start))))
-    | _ => Vundef
-    end
-  else Vundef.
-
-
-Definition extfs stop start v :=
-  if (Z.leb start stop)
-       && (Z.geb start Z.zero)
-       && (Z.ltb stop Int.zwordsize)
-  then
-    let stop' := Z.add stop Z.one in
-    match v with
-    | Vint w =>
-      Vint (Int.shr (Int.shl w (Int.repr (Z.sub Int.zwordsize stop'))) (Int.repr (Z.sub Int.zwordsize (Z.sub stop' start))))
-    | _ => Vundef
-    end
-  else Vundef.
-
-Definition extfzl stop start v :=
-  if (Z.leb start stop)
-       && (Z.geb start Z.zero)
-       && (Z.ltb stop Int64.zwordsize)
-  then
-    let stop' := Z.add stop Z.one in
-    match v with
-    | Vlong w =>
-      Vlong (Int64.shru' (Int64.shl' w (Int.repr (Z.sub Int64.zwordsize stop'))) (Int.repr (Z.sub Int64.zwordsize (Z.sub stop' start))))
-    | _ => Vundef
-    end
-  else Vundef.
-
-
-Definition extfsl stop start v :=
-  if (Z.leb start stop)
-       && (Z.geb start Z.zero)
-       && (Z.ltb stop Int64.zwordsize)
-  then
-    let stop' := Z.add stop Z.one in
-    match v with
-    | Vlong w =>
-      Vlong (Int64.shr' (Int64.shl' w (Int.repr (Z.sub Int64.zwordsize stop'))) (Int.repr (Z.sub Int64.zwordsize (Z.sub stop' start))))
-    | _ => Vundef
-    end
-  else Vundef.
-
-
 (** Comparisons *)
 
 Section COMPARISONS.
