mppa_k1c/Asm.v
@@ -23,6 +23,7 @@ Require Import AST.
 Require Import Integers.
 Require Import Floats.
 Require Import Values.
+Require Import ExtValues.
 Require Import Memory.
 Require Import Events.
 Require Import Globalenvs.
