mppa_k1c/ExtValues.v
@@ -1,0 +1,57 @@
+Require Import Coqlib.
+Require Import Integers.
+Require Import Values.
+
+Definition extfz stop start v :=
+  if (Z.leb start stop)
+       && (Z.geb start Z.zero)
+       && (Z.ltb stop Int.zwordsize)
+  then
+    let stop' := Z.add stop Z.one in
+    match v with
+    | Vint w =>
+      Vint (Int.shru (Int.shl w (Int.repr (Z.sub Int.zwordsize stop'))) (Int.repr (Z.sub Int.zwordsize (Z.sub stop' start))))
+    | _ => Vundef
+    end
+  else Vundef.
+
+
+Definition extfs stop start v :=
+  if (Z.leb start stop)
+       && (Z.geb start Z.zero)
+       && (Z.ltb stop Int.zwordsize)
+  then
+    let stop' := Z.add stop Z.one in
+    match v with
+    | Vint w =>
+      Vint (Int.shr (Int.shl w (Int.repr (Z.sub Int.zwordsize stop'))) (Int.repr (Z.sub Int.zwordsize (Z.sub stop' start))))
+    | _ => Vundef
+    end
+  else Vundef.
+
+Definition extfzl stop start v :=
+  if (Z.leb start stop)
+       && (Z.geb start Z.zero)
+       && (Z.ltb stop Int64.zwordsize)
+  then
+    let stop' := Z.add stop Z.one in
+    match v with
+    | Vlong w =>
+      Vlong (Int64.shru' (Int64.shl' w (Int.repr (Z.sub Int64.zwordsize stop'))) (Int.repr (Z.sub Int64.zwordsize (Z.sub stop' start))))
+    | _ => Vundef
+    end
+  else Vundef.
+
+
+Definition extfsl stop start v :=
+  if (Z.leb start stop)
+       && (Z.geb start Z.zero)
+       && (Z.ltb stop Int64.zwordsize)
+  then
+    let stop' := Z.add stop Z.one in
+    match v with
+    | Vlong w =>
+      Vlong (Int64.shr' (Int64.shl' w (Int.repr (Z.sub Int64.zwordsize stop'))) (Int.repr (Z.sub Int64.zwordsize (Z.sub stop' start))))
+    | _ => Vundef
+    end
+  else Vundef.
